pulse/lib/pulse/lib/Pulse.Lib.Slice.fst
@@ -184,7 +184,7 @@ fn split (#t: Type) (s: slice t) (#p: perm) (i: SZ.t)
 {
     unfold_pts_to s #p v;
     Seq.lemma_split v (SZ.v i);
-    let elt' = AP.split s.elt #p #v i;
+    let elt' = AP.split s.elt #p i;
     let s1 = {
         elt = s.elt;
         len = i;
@@ -209,6 +209,27 @@ fn join (#t: Type) (s1: slice t) (#p: perm) (#v1: Seq.seq t) (s2: slice t) (#v2:
     unfold_pts_to s2 #p v2;
     AP.join s1.elt s2.elt;
     fold_pts_to s #p (Seq.append v1 v2)
+}
+
+fn subslice #t (s: slice t) #p (i j: SZ.t) (#v: erased (Seq.seq t) { SZ.v i <= SZ.v j /\ SZ.v j <= Seq.length v })
+  requires pts_to s #p v
+  returns res: slice t
+  ensures pts_to res #p (Seq.slice v (SZ.v i) (SZ.v j)) ** subslice_rest res s p i j v
+{
+  unfold_pts_to s #p v;
+  let elt' = AP.split s.elt i;
+  let elt'' = AP.ghost_split elt' (SZ.sub j i);
+  let s1 = hide { elt = s.elt; len = i };
+  let s2 = hide { elt = elt'; len = SZ.sub s.len i };
+  fold is_split s s1 s2;
+  let res = hide { elt = elt'; len = SZ.sub j i };
+  let s3 = hide { elt = elt''; len = SZ.sub s.len j };
+  fold is_split s2 res s3;
+  fold_pts_to s1 #p (Seq.slice v 0 (SZ.v i));
+  fold_pts_to res #p (Seq.slice v (SZ.v i) (SZ.v j));
+  fold_pts_to s3 #p (Seq.slice v (SZ.v j) (Seq.length v));
+  fold subslice_rest;
+  ({ elt = elt'; len = SZ.sub j i })
 }
 
 fn copy
